@prefix rdfs:    <http://www.w3.org/2000/01/rdf-schema#> .
@prefix rdf:     <http://www.w3.org/1999/02/22-rdf-syntax-ns#> .
@prefix dc:      <http://purl.org/dc/elements/1.1/> .
@prefix dcterms: <http://purl.org/dc/terms/> .
@prefix event:   <http://purl.org/NET/c4dm/event.owl#> .
@prefix foaf:    <http://xmlns.com/foaf/0.1/> .
@prefix skos:    <https://www.w3.org/2009/08/skos-reference/skos#> .
@prefix oa:      <http://www.w3.org/ns/oa#> .
@prefix frbr:    <http://purl.org/vocab/frbr/core#> .
@prefix mAnnot:  <https://raw.githubusercontent.com/DomesticBeethoven/dbsite/gh-pages/ontology/music-annotation-ontology.ttl> .

mAnnot:MusicalIdea a rdfs:Class ;
   rdfs:subClassOf frbr:Work ;
   rdfs:label "MusicalIdea" ;
   rdfs:comment "Analogous to frbr:work, but on a local level, as an element of a larger piece. An abstract entity that refers to the musical thought behind a musical structure, especially a recurring one." .

mAnnot:MusicalMaterial a rdfs:Class ;
   rdfs:subClassOf frbr:Expression ;
   rdfs:label "MusicalMaterial" ;
 	 rdfs:comment "The musical concept behind a musical Extract, independent of its various expressions in different arrangements or recordings (or, in a variation set, within a single variation). The realization of a MusicalIdea." .

mAnnot:Extract a rdfs:Class ;
   rdfs:subClassOf frbr:Expression ;
   rdfs:label "Extract" ;
 	 rdfs:comment "A portion of music, independent of its manifestation in a particular edition, or its realization in any individual performance or media format." .

mAnnot:Selection a rdfs:Class ;
   rdfs:subClassOf frbr:Manifestation ;
   rdfs:label "Selection" ;
 	 rdfs:comment "A collection of UUIDs that comprise a single musical object, at any level, within a single resource." .

 mAnnot:setting a rdf:Property ;
   rdfs:domain mAnnot:Extract ;
   rdfs:range mAnnot:Selection ;
   rdfs:comment "A setting of an Extract. The relationship that holds between an Extract and the individual Selections that comprise it. Similar to frbr:manifestation, but designed especially for this extended FRBR class. ".

mAnnot:settingOf a rdf:Property ;
   rdfs:domain mAnnot:Selection ;
   rdfs:range mAnnot:Extract ;
   rdfs:comment "The Extract that the Selection is a setting of. Similar to frbr:manifestationOf, but designed especially for this extended FRBR class.".

mAnnot:absenceSelection a rdfs:Class ;
  rdfs:subClassOf mAnnot:Selection ;
  rdfs:comment "A point marker that combines with an AbsenceQualification value (e.g., 'before') to indicate the location of an addition or abridgment relative to another version of the same work" .

mAnnot:absenceQualifier a rdf:Property ;
  rdfs:domain mAnnot:absenceSelection ;
  rdfs:range mAnnot:AbsenceQualification .

mAnnot:absenceQualification a rdfs:Class ;
  rdfs:domain mAnnot:absenceQualifier .

mAnnot:observing a oa:motivation ;
  skos:broader oa:describing ;
  skos:prefLabel "observing" ;
  rdfs:label "observing" ;
  rdfs:comment "A type of annotation making an observation (rather than a comment), often for purposes of comparison" .

mAnnot:comparing a oa:motivation ;
  skos:broader oa:describing ;
  skos:prefLabel "comparing" ;
  rdfs:label "comparing" ;
  rdfs:comment "A type of annotation that makes a comparison of two or more versions or Extracts, often for purposes of scholarly commentary" .

mAnnot:commenting a oa:motivation ;
  skos:prefLabel "commenting" ;
  rdfs:label "commenting" ;
  rdfs:comment "A type of annotation that makes a comment on musical structure or another annotation, often used to enrich Observation descriptions with historical background and analytical reflections informed by academic research. Includes pointers to external sources and references" .
