@prefix rdfs:    <http://www.w3.org/2000/01/rdf-schema#> .
@prefix dc:      <http://purl.org/dc/elements/1.1/> .
@prefix dcterms: <http://purl.org/dc/terms/> .
@prefix event:   <http://purl.org/NET/c4dm/event.owl#> .
@prefix foaf:    <http://xmlns.com/foaf/0.1/> .
@prefix skos:    <https://www.w3.org/2009/08/skos-reference/skos#> .
@prefix oa:      <http://www.w3.org/ns/oa#> .
@prefix frbr:    <http://purl.org/vocab/frbr/core#> .

bithTerms:MusicalIdea a rdfs:Class ;
   rdfs:subClassOf frbr:Work .
   rdfs:label "MusicalIdea" ;
   rdfs:comment "Similar to frbr:work, a MusicalIdea is highest abstraction of "

bithTerms:MusicalMaterial a rdfs:Class ;
   rdfs:subClassOf frbr:Expression ;
   rdfs:label "MusicalMaterial" ;
 	 rdfs:comment "An object which identifies two or more passages from different versions as parallel." .

bithTerms:Extract a rdfs:Class ;
   rdfs:subClassOf frbr:Expression ;
   rdfs:label "Extract" ;
 	 rdfs:comment "A portion of music, without regard to notation or performance, independent of media format." .

bithTerms:Selection ;
   rdfs:subClassOf frbr:Manifestation ;
   rdfs:label "Selection" ;
 	 rdfs:comment "A collection of UUIDs that comprise a single musical object, at any level, within a single resource." .

bithTerms:AbsenceSelection a rdfs:Class ;
  rdfs:subClassOf bithTerms:Selection .

bithTerms:absenceQualifier a rdf:Property ;
  rdfs:domain bithTerms:absenceSelection ;
  rdfs:range bithTerms:AbsenceQualification .

bithTerms:AbsenceQualification a rdfs:Class ;
  rdfs:domain bithTerms:absenceQualifier .

bithTerms:observing a oa:motivation ;
  skos:broader oa:describing ;
  skos:prefLabel "observing" ;
  rdfs:label "observing" ;
  rdfs:comment "making an observation (rather than a comment), often for purposes of comparison" .

  bithTerms:comparing a oa:motivation ;
    skos:broader oa:describing ;
    skos:prefLabel "comparing" ;
    rdfs:label "comparing" ;
    rdfs:comment "making a comparison of two or more versions or Extracts" .




Version ontology

--------

https://domestic-beethoven.eu/ontologies/musical-object-layer#MusicalMaterial

https://github.com/motools/musicontology/blob/master/rdf/musicontology.n3
